FOL/Semantics.lean
@@ -1,4 +1,5 @@
 import FOL.Binders
+import FOL.Definition
 import FOL.FunctionUpdateIte
 import FOL.Tactics
 
@@ -52,20 +53,38 @@ instance (D : Type) [Inhabited D] : Inhabited (VarAssignment D) :=
 -/
 def Holds
   (D : Type)
-  (I : Interpretation D) :
-  VarAssignment D → Formula → Prop
-  | V, pred_const_ X xs => I.pred_const_ X (xs.map V)
-  | V, pred_var_ X xs => I.pred_var_ X (xs.map V)
-  | V, eq_ x y => V x = V y
+  (I : Interpretation D)
+  (V : VarAssignment D) : Env → Formula → Prop
+  | _, pred_const_ X xs => I.pred_const_ X (xs.map V)
+  | _, pred_var_ X xs => I.pred_var_ X (xs.map V)
+  | _, eq_ x y => V x = V y
   | _, true_ => True
   | _, false_ => False
-  | V, not_ phi => ¬ Holds D I V phi
-  | V, imp_ phi psi => Holds D I V phi → Holds D I V psi
-  | V, and_ phi psi => Holds D I V phi ∧ Holds D I V psi
-  | V, or_ phi psi => Holds D I V phi ∨ Holds D I V psi
-  | V, iff_ phi psi => Holds D I V phi ↔ Holds D I V psi
-  | V, forall_ x phi => ∀ d : D, Holds D I (Function.updateIte V x d) phi
-  | V, exists_ x phi => ∃ d : D, Holds D I (Function.updateIte V x d) phi
+  | E, not_ phi => ¬ Holds D I V E phi
+  | E, imp_ phi psi =>
+    have : sizeOf psi < sizeOf (imp_ phi psi) := by simp
+    Holds D I V E phi → Holds D I V E psi
+  | E, and_ phi psi =>
+    have : sizeOf psi < sizeOf (and_ phi psi) := by simp
+    Holds D I V E phi ∧ Holds D I V E psi
+  | E, or_ phi psi =>
+    have : sizeOf psi < sizeOf (or_ phi psi) := by simp
+    Holds D I V E phi ∨ Holds D I V E psi
+  | E, iff_ phi psi =>
+    have : sizeOf psi < sizeOf (iff_ phi psi) := by simp
+    Holds D I V E phi ↔ Holds D I V E psi
+  | E, forall_ x phi =>
+    have : sizeOf phi < sizeOf (forall_ x phi) := by simp
+    ∀ d : D, Holds D I (Function.updateIte V x d) E phi
+  | E, exists_ x phi =>
+    have : sizeOf phi < sizeOf (exists_ x phi) := by simp
+    ∃ d : D, Holds D I (Function.updateIte V x d) E phi
+  | ([] : Env), def_ _ _ => False
+  | d :: E, def_ name args =>
+    if name = d.name ∧ args.length = d.args.length
+    then Holds D I (Function.updateListIte V d.args (List.map V args)) E d.q
+    else Holds D I V E (def_ name args)
+termination_by _ E phi => (E.length, phi)
 
 
 /--
@@ -74,139 +93,189 @@ def Holds
   Formula.isValid F := True if and only if F evaluates to True in every combination of domain of discourse, interpretation and variable assignment.
 -/
 def Formula.IsValid (F : Formula) : Prop :=
-  ∀ (D : Type) (I : Interpretation D) (V : VarAssignment D), Holds D I V F
+  ∀ (D : Type) (I : Interpretation D) (V : VarAssignment D) (E : Env), Holds D I V E F
 
 
 theorem Holds_coincide_Var
   (D : Type)
   (I : Interpretation D)
   (V V' : VarAssignment D)
+  (E : Env)
   (F : Formula)
   (h1 : ∀ v : VarName, isFreeIn v F → V v = V' v) :
-  Holds D I V F ↔ Holds D I V' F :=
+  Holds D I V E F ↔ Holds D I V' E F :=
   by
-  induction F generalizing V V'
-  case pred_const_ X xs | pred_var_ X xs =>
-    unfold isFreeIn at h1
+  induction E generalizing F V V'
+  all_goals
+    induction F generalizing V V'
+    case pred_const_ X xs | pred_var_ X xs =>
+      unfold isFreeIn at h1
 
-    unfold Holds
-    congr! 1
-    simp only [List.map_eq_map_iff]
-    exact h1
-  case eq_ x y =>
-    unfold isFreeIn at h1
-    simp at h1
+      simp only [Holds]
+      congr! 1
+      simp only [List.map_eq_map_iff]
+      exact h1
+    case eq_ x y =>
+      unfold isFreeIn at h1
+      simp at h1
 
-    unfold Holds
-    cases h1
-    case intro h1_left h1_right =>
-      simp only [h1_left, h1_right]
-  case true_ | false_ =>
+      simp only [Holds]
+      cases h1
+      case intro h1_left h1_right =>
+        simp only [h1_left, h1_right]
+    case true_ | false_ =>
+      simp only [Holds]
+    case not_ phi phi_ih =>
+      simp only [Holds]
+      congr! 1
+      exact phi_ih V V' h1
+    case
+        imp_ phi psi phi_ih psi_ih
+      | and_ phi psi phi_ih psi_ih
+      | or_ phi psi phi_ih psi_ih
+      | iff_ phi psi phi_ih psi_ih =>
+      unfold isFreeIn at h1
+
+      simp only [Holds]
+      congr! 1
+      · apply phi_ih V V'
+        intro v a1
+        apply h1
+        left
+        exact a1
+      · apply psi_ih V V'
+        intro v a1
+        apply h1
+        right
+        exact a1
+    case forall_ x phi phi_ih | exists_ x phi phi_ih =>
+      unfold isFreeIn at h1
+      simp at h1
+
+      simp only [Holds]
+      first | apply forall_congr' | apply exists_congr
+      intro d
+      apply phi_ih
+      intro v a1
+      simp only [Function.updateIte]
+      split_ifs
+      case _ c1 =>
+        rfl
+      case _ c1 =>
+        exact h1 v c1 a1
+
+  case nil.def_ X xs =>
     unfold Holds
     rfl
-  case not_ phi phi_ih =>
-    unfold Holds
-    congr! 1
-    exact phi_ih V V' h1
-  case
-      imp_ phi psi phi_ih psi_ih
-    | and_ phi psi phi_ih psi_ih
-    | or_ phi psi phi_ih psi_ih
-    | iff_ phi psi phi_ih psi_ih =>
+
+  case cons.def_ hd tl ih X xs =>
     unfold isFreeIn at h1
 
-    unfold Holds
-    congr! 1
-    · apply phi_ih V V'
-      intro v a1
-      apply h1
-      left
-      exact a1
-    · apply psi_ih V V'
-      intro v a1
-      apply h1
-      right
-      exact a1
-  case forall_ x phi phi_ih | exists_ x phi phi_ih =>
-    unfold isFreeIn at h1
-    simp at h1
-
-    unfold Holds
-    first | apply forall_congr' | apply exists_congr
-    intro d
-    apply phi_ih
-    intro v a1
-    simp only [Function.updateIte]
+    simp only [Holds]
     split_ifs
-    case _ c1 =>
-      rfl
-    case _ c1 =>
-      exact h1 v c1 a1
+    case inl c1 =>
+      apply ih
+      intro v a1
+      simp only [isFreeIn_iff_mem_freeVarSet v hd.q] at a1
+      
+      have s2 : v ∈ List.toFinset hd.args
+      apply Finset.mem_of_subset hd.nf a1
+
+      apply Function.updateListIte_fun_coincide_mem_eq_len V V' hd.args xs v h1
+      · simp only [List.mem_toFinset] at s2
+        exact s2
+      · cases c1
+        case _ c1_left c1_right =>
+          simp only [eq_comm]
+          exact c1_right
+    case inr c1 =>
+      apply ih
+      unfold isFreeIn
+      exact h1
 
 
 theorem Holds_coincide_PredVar
   (D : Type)
   (I I' : Interpretation D)
   (V : VarAssignment D)
+  (E : Env)
   (F : Formula)
   (h1 : I.pred_const_ = I'.pred_const_)
   (h2 : ∀ (P : PredName) (ds : List D),
     predVarOccursIn P ds.length F →
       (I.pred_var_ P ds ↔ I'.pred_var_ P ds)) :
-  Holds D I V F ↔ Holds D I' V F :=
+  Holds D I V E F ↔ Holds D I' V E F :=
   by
-  induction F generalizing V
-  case pred_const_ X xs =>
-    unfold Holds
-    simp only [h1]
-  case pred_var_ X xs =>
-    unfold predVarOccursIn at h2
-    simp at h2
+  induction E generalizing F V
+  all_goals
+    induction F generalizing V
+    case pred_const_ X xs =>
+      unfold Holds
+      simp only [h1]
+    case pred_var_ X xs =>
+      unfold predVarOccursIn at h2
+      simp at h2
 
-    unfold Holds
-    apply h2
-    · rfl
-    · simp
-  case eq_ x y =>
-    unfold Holds
-    rfl
-  case true_ | false_ =>
-    unfold Holds
-    rfl
-  case not_ phi phi_ih =>
-    unfold predVarOccursIn at h2
+      unfold Holds
+      apply h2
+      · rfl
+      · simp
+    case eq_ x y =>
+      unfold Holds
+      rfl
+    case true_ | false_ =>
+      unfold Holds
+      rfl
+    case not_ phi phi_ih =>
+      unfold predVarOccursIn at h2
 
-    unfold Holds
-    congr! 1
-    exact phi_ih V h2
-  case
-      imp_ phi psi phi_ih psi_ih
-    | and_ phi psi phi_ih psi_ih
-    | or_ phi psi phi_ih psi_ih
-    | iff_ phi psi phi_ih psi_ih =>
-    unfold predVarOccursIn at h2
+      unfold Holds
+      congr! 1
+      exact phi_ih V h2
+    case
+        imp_ phi psi phi_ih psi_ih
+      | and_ phi psi phi_ih psi_ih
+      | or_ phi psi phi_ih psi_ih
+      | iff_ phi psi phi_ih psi_ih =>
+      unfold predVarOccursIn at h2
 
-    unfold Holds
-    congr! 1
-    · apply phi_ih
+      simp only [Holds]
+      congr! 1
+      · apply phi_ih
+        intro P ds a1
+        apply h2
+        left
+        exact a1
+      · apply psi_ih
+        intro P ds a1
+        apply h2
+        right
+        exact a1
+    case forall_ x phi phi_ih | exists_ x phi phi_ih =>
+      unfold predVarOccursIn at h2
+
+      unfold Holds
+      first | apply forall_congr' | apply exists_congr
+      intro d
+      exact phi_ih (Function.updateIte V x d) h2
+
+  case nil.def_ X xs =>
+    simp only [Holds]
+
+  case cons.def_ hd tl ih X xs =>
+    simp only [Holds]
+    split_ifs
+    case inl c1 =>
+      apply ih
       intro P ds a1
       apply h2
-      left
-      exact a1
-    · apply psi_ih
+      sorry
+    case inr c1 =>
+      apply ih
       intro P ds a1
-      apply h2
-      right
-      exact a1
-  case forall_ x phi phi_ih | exists_ x phi phi_ih =>
-    unfold predVarOccursIn at h2
+      unfold predVarOccursIn at a1
+      contradiction
 
-    unfold Holds
-    first | apply forall_congr' | apply exists_congr
-    intro d
-    exact phi_ih (Function.updateIte V x d) h2
-
-
-#lint
+--#lint
 
 end FOL
