FOL/Definition.lean
@@ -1,0 +1,52 @@
+import FOL.Formula
+import FOL.Binders
+import FOL.Tactics
+
+
+namespace FOL
+
+open Formula
+
+
+structure Definition : Type :=
+(name : DefName)
+(args : List VarName)
+(q : Formula)
+(nodup : args.Nodup)
+(nf : q.freeVarSet ⊆ args.toFinset)
+deriving DecidableEq
+
+
+def Env : Type := List Definition
+
+instance : Membership Definition Env :=
+  inferInstanceAs (Membership Definition (List Definition))
+
+
+def Formula.all_def_in_env (E : Env) : Formula → Prop
+| pred_const_ _ _ => True
+| pred_var_ _ _ => True
+| eq_ _ _ => True
+| true_ => True
+| false_ => True
+| not_ phi => phi.all_def_in_env E
+| imp_ phi psi =>
+    phi.all_def_in_env E ∧
+    psi.all_def_in_env E
+| and_ phi psi =>
+    phi.all_def_in_env E ∧
+    psi.all_def_in_env E
+| or_ phi psi =>
+    phi.all_def_in_env E ∧
+    psi.all_def_in_env E
+| iff_ phi psi =>
+    phi.all_def_in_env E ∧
+    psi.all_def_in_env E
+| forall_ _ phi => phi.all_def_in_env E
+| exists_ _ phi => phi.all_def_in_env E
+| def_ X xs =>
+  ∃ (d : Definition), d ∈ E ∧ X = d.name ∧ xs.length = d.args.length
+
+
+def Env.nodup_ : Env → Prop :=
+  List.Pairwise (fun (d1 d2 : Definition) => d1.name = d2.name → d1.args.length = d2.args.length → False)
